Correctness.v
@@ -7,38 +7,127 @@ Require Import List.
 
 Import ListNotations.
 
+Import Lia.
+
 Notation "Σ ;;; Γ |- t1 ⇓ t2 " := (WcbvEval.eval Σ Γ t1 t2) (at level 50).
 Notation "T⟦ e ⟧ Σ " := (expr_to_term Σ e) (at level 40).
 
 Import InterpreterEnvList.
 
-Theorem expr_to_term_sound n ρ Σ1 Σ2 (Γ:=[]) (e : expr) (t : term) (v : val) :
-  Σ2 ;;; Γ |- T⟦e⟧Σ1 ⇓ t ->
-  expr_eval_i n Σ1 ρ e = Ok v ->
+Lemma map_env_list_size {A B} (f : Ast.name -> A -> B) (ρ : env A) :
+  length (map_env_list f ρ) = size ρ.
+Proof.
+Admitted.
+
+Lemma from_option_indep {A} (o : option A) d  d' v :
+  o = Some v -> from_option o d = from_option o d'.
+Proof.
+  intros;subst;easy.
+Qed.
+
+Lemma lookup_i_norec_some {A} {ρ : env A} {n : nat} :
+  n < size ρ ->
+  exists v, lookup_i_norec ρ n = Some v.
+Proof.
+  revert dependent n.
+  induction ρ;intros n1 Hlt.
+  + eexists;easy.
+  + simpl in *. destruct (Nat.eqb n1 0) eqn:Hn1.
+    * eexists;reflexivity.
+    * assert (Hn2 : exists n2, n1 = S n2) by
+          (destruct n1 as [ | n2]; tryfalse; exists n2; reflexivity).
+      destruct Hn2 as [n2 Heq_n2]. replace (n1-1) with n2 by lia.
+      subst. apply Lt.lt_S_n in Hlt.
+      (* assert (n1=0) by (apply EqNat.beq_nat_eq; easy). subst. *)
+Admitted.
+
+Lemma inst_env_i_in ρ n :
+  n < size ρ ->
+  exists v, lookup_i ρ n = Some v /\ inst_env_i ρ (eRel n) = from_val_i v.
+Proof.
+  intros Hlt.
+  revert dependent n.
+  induction ρ;intros n1 Hlt.
+  + inversion Hlt.
+  + destruct (Nat.eqb n1 0) eqn:Hn1.
+    * eexists. split.
+      ** simpl. rewrite Hn1.
+         reflexivity.
+      ** simpl in *. unfold inst_env_i,subst_env_i. simpl.
+         assert (n1=0) by (apply EqNat.beq_nat_eq; easy).
+         subst. simpl. admit.
+    * assert (Hn2 : exists n2, n1 = S n2) by (destruct n1 as [ | n2]; tryfalse; exists n2; reflexivity).
+      destruct Hn2 as [n2 Heq_n2]. replace (n1-1) with n2 by lia. subst. simpl in Hlt.
+      apply Lt.lt_S_n in Hlt.
+      specialize (IHρ _ Hlt). destruct IHρ as [v HH]. destruct HH as [H1 H2].
+      exists v. split.
+      ** simpl in *. replace (n2 - 0) with n2 by lia. assumption.
+      ** specialize (lookup_i_norec_some Hlt) as Hlookup.
+         destruct Hlookup.
+         simpl in *. unfold inst_env_i,subst_env_i in *. simpl in *.
+         rewrite <- H2. replace (n2 - 0) with n2 by lia.
+         eapply from_option_indep.
+
+  (*        apply nth_indep. rewrite map_env_list_size. *)
+  (*        assumption. *)
+  (* + simpl in *. *)
+Admitted.
+
+Lemma inst_env_i_notin ρ n :
+  size ρ <= n -> lookup_i ρ n = None.
+Proof.
+  Admitted.
+
+Lemma Wcbv_from_value_value v Σ : WcbvEval.value (T⟦ from_val_i v⟧Σ).
+Proof.
+Admitted.
+
+(* This should from the fact that ⇓ is deterministic and
+   the fact that value evaluates to itself, but the fact that
+   ⇓ is deterministic is not yet proved in Template Coq *)
+Lemma Wcbv_eval_value_determ Σ (Γ:=[]) t1 t2 :
+  WcbvEval.value t1 -> Σ ;;; Γ |- t1 ⇓ t2 -> t1 = t2.
+Proof.
+  Admitted.
+
+
+Theorem expr_to_term_sound n ρ Σ1 Σ2 (Γ:=[]) (e1 e2 : expr) (t : term) (v : val) :
+  inst_env_i ρ e1 = e2 ->
+  Σ2 ;;; Γ |- T⟦e2⟧Σ1 ⇓ t ->
+  expr_eval_i n Σ1 ρ e1 = Ok v ->
   t = T⟦from_val_i v⟧Σ1.
 Proof.
   revert dependent v.
   revert dependent t.
   revert dependent ρ.
-  revert dependent n.
-  induction e using expr_ind_case;intros n1 ρ t1 v.
-  + (* eRel*)
-    (*This case is trivial because we assume that we deal with closed terms by putting Γ = [] *)
-    intros HT He. simpl in *. destruct n1; tryfalse. autounfold with facts in *.
-    simpl in *.
-    destruct (lookup_i ρ n) eqn:Hlookup;tryfalse. simpl in He;inversion He;subst.
-    inversion HT;subst;simpl in *. inversion isdecl. inversion isdecl.
-  + (* eVar *)
-    (* This case is trivial because we only consider terms with de Bruijn indices *)
-    intros HT He. destruct n1; tryfalse.
-  + (* eLambda *)
-    intros HT He. destruct n1; tryfalse.
-    autounfold with facts in *. simpl in HT. simpl in He.
-    inversion He. simpl. inversion HT. subst.
-    destruct ρ.
-    * simpl. repeat f_equal. apply subst_env_i_empty.
-    * simpl.
-      destruct (n0 =? n).
-      ** f_equal.
+  revert dependent e2.
+  revert dependent e1.
+  induction n.
+  - intros;tryfalse.
+  - intros e1 e2 ρ t v Henv HT He.
+    destruct e1.
+    + (* eRel*)
+      autounfold with facts in *. simpl in *.
+      destruct (lookup_i ρ n0) eqn:Hlookup;tryfalse. simpl in He;inversion He;subst.
+
+      assert (Hn0 : n0 < size ρ \/ size ρ <= n0) by lia.
+      destruct Hn0 as [Hlt | Hge].
+      * destruct (inst_env_i_in _ _ Hlt) as [v1 HH].
+        destruct HH as [H1 H2].
+        assert (v1 = v) by congruence. subst.
+        rewrite H2 in HT.
+        symmetry.
+        eapply Wcbv_eval_value_determ;
+        [apply Wcbv_from_value_value | eassumption ].
+      * specialize (inst_env_i_notin _ _ Hge) as Hnone;tryfalse.
+    + (* eVar *)
+      (* This case is trivial because we only consider terms with de Bruijn indices *)
+      destruct n0; tryfalse.
+    + (* eLambda *)
+      autounfold with facts in *. simpl in HT. simpl in He.
+      inversion He. simpl. inversion HT. subst.
+      destruct ρ.
+      * simpl. repeat f_equal. apply subst_env_i_empty.
+      * simpl. f_equal.
 
 Admitted.
